

# MATRICES AND CALCULUS ASSIGNMENT

Sec 251097  
Santhosh -A  
It - E

### Module-3

#### Assignment-Questions:

1. Find the directional derivative of  $\phi = 2xy + z^2$  at the point  $(1, -1, 3)$  in the direction of  $\vec{i} + 2\vec{j} + 2\vec{k}$ .

Let:

$$D = \vec{\nabla} \cdot \phi \cdot \frac{\vec{a}}{|\vec{a}|} \quad \text{--- (1)}$$

given:

$$\phi = 2xy + z^2, \quad \vec{a} = \vec{i} + 2\vec{j} + 2\vec{k}$$

$$\vec{\nabla} \cdot \phi = \vec{i} \frac{\partial \phi}{\partial x} + \vec{j} \frac{\partial \phi}{\partial y} + \vec{k} \frac{\partial \phi}{\partial z}$$

$$\frac{\partial \phi}{\partial x} = 2y$$

$$\frac{\partial \phi}{\partial y} = 2x$$

$$\frac{\partial \phi}{\partial z} = 2z$$

$$\vec{\nabla} \cdot \phi = \vec{i} 2y + \vec{j} 2x + \vec{k} 2z$$

Put  $(1, -1, 3)$  points

$$\vec{\nabla} \cdot \phi = -2\vec{i} + 2\vec{j} + 6\vec{k}$$

$$\textcircled{1} \Rightarrow D = \vec{\nabla} \cdot \phi \cdot \frac{\vec{a}}{|\vec{a}|}$$

$$D = -2\vec{i} + 2\vec{j} + 6\vec{k} \cdot \frac{\vec{i} + 2\vec{j} + 2\vec{k}}{\sqrt{(1)^2 + (2)^2 + (2)^2}}$$

$$D = \frac{-2 + 4 + 12}{\sqrt{9}}$$

$$D = \frac{14}{3}$$

2. Find the angle between the surfaces  $x^2 - y^2 - z^2 = 11$  and  $xy + yz - zx - 18 = 0$  at point  $(6, 4, 3)$

Given:

$$\phi_1 \Rightarrow x^2 - y^2 - z^2 - 11 = 0$$

$$\phi_2 \Rightarrow xy + yz - zx - 18 = 0$$

WKT:

$$\cos \theta = \frac{\vec{\nabla} \phi_1 \cdot \vec{\nabla} \phi_2}{|\vec{\nabla} \phi_1| |\vec{\nabla} \phi_2|} \quad \text{--- (1)}$$

$$\vec{\nabla} \phi_1 = \vec{i} \frac{\partial \phi_1}{\partial x} + \vec{j} \frac{\partial \phi_1}{\partial y} + \vec{k} \frac{\partial \phi_1}{\partial z}$$

$$\nabla \phi_1 = \vec{i} (2x) + \vec{j} (-2y) + \vec{k} (-2z)$$

$$\nabla \phi_1 = 12\vec{i} - 8\vec{j} - 6\vec{k} \quad \text{--- (2) } (\because \text{Put } (6, 4, 3))$$

$$\nabla \phi_2 = \vec{i} \frac{\partial \phi_2}{\partial x} + \vec{j} \frac{\partial \phi_2}{\partial y} + \vec{k} \frac{\partial \phi_2}{\partial z}$$

$$\nabla \phi_2 = \vec{i} (y - z) + \vec{j} (x + z) + \vec{k} (y - x)$$

Put  $(6, 4, 3)$  points

$$\nabla \phi_2 = \vec{i} + 9\vec{j} - 2\vec{k} \quad \text{--- (3)}$$

Substituting (3) & (2) in (1) we get

$$\cos \theta = \frac{(12\vec{i} - 8\vec{j} - 6\vec{k}) \cdot (\vec{i} + 9\vec{j} - 2\vec{k})}{(\sqrt{(12)^2 + (-8)^2 + (-6)^2}) (\sqrt{(1)^2 + (9)^2 + (-2)^2})}$$

$$\cos \theta = \frac{12 - 72 + 12}{\sqrt{244} \sqrt{86}}$$

$$\theta = \cos^{-1} \left( \frac{-48}{\sqrt{244} \sqrt{86}} \right) \quad \text{or} \quad \cos^{-1} \left( \frac{-48}{\sqrt{21000}} \right)$$

3. Find the scalar point function whose gradient is  
 $(2xy - z^2)\vec{i} + (2yz + x^2)\vec{j} + (y^2 - 2zx)\vec{k}$

Let:

$$F = (2xy - z^2)\vec{i} + (2yz + x^2)\vec{j} + (y^2 - 2zx)\vec{k}$$

$$\nabla\phi = \vec{i} \frac{\partial\phi}{\partial x} + \vec{j} \frac{\partial\phi}{\partial y} + \vec{k} \frac{\partial\phi}{\partial z}$$

Equating the both coefficient  $\vec{i}, \vec{j}, \vec{k}$

$$\frac{\partial\phi}{\partial x} = 2xy - z^2 \quad \text{--- (1)}$$

$$\frac{\partial\phi}{\partial y} = 2yz + x^2 \quad \text{--- (2)}$$

$$\frac{\partial\phi}{\partial z} = y^2 - 2zx \quad \text{--- (3)}$$

Integrating with respect to  $x$  in (1)

$$\int d\phi = \int (2xy - z^2) dx$$

$$\phi = \frac{2x^2y}{2} - z^2x$$

$$\phi = x^2y - xz^2 + C \quad \text{--- (4)}$$

Integrating w.r to  $y$  in (2)

$$\int d\phi = \int (2yz + x^2) dy$$

$$\phi = \frac{2y^2}{2}z + x^2y$$

$$\phi = y^2z + x^2y + C \quad \text{--- (5)}$$

Integrating w.r to  $z$  in (3)

$$\int d\phi = \int (y^2 - 2zx) dz$$

$$\phi = zy^2 - \frac{2z^2x}{2}$$

$$= zy^2 - xz^2 + C \quad \text{--- (5)}$$

From (4), (5), (6)

$$\phi = x^2y + y^2z - z^2x + C$$

4. Show that  $\vec{F} = (y^2 \cos x + z^3) \vec{i} + (2y \sin x - 4) \vec{j} + 3xz^2 \vec{k}$  is irrotational and find its scalar potential.

WKT:

$$\nabla \times \vec{F} = \begin{vmatrix} \vec{i} & \vec{j} & \vec{k} \\ \frac{\partial}{\partial x} & \frac{\partial}{\partial y} & \frac{\partial}{\partial z} \\ y^2 \cos x + z^3 & 2y \sin x - 4 & 3xz^2 \end{vmatrix}$$

$$= \vec{i} \left[ \frac{\partial}{\partial y} (3xz^2) - \frac{\partial}{\partial z} (2y \sin x - 4) \right] - \vec{j} \left[ \frac{\partial}{\partial x} (3xz^2) - \frac{\partial}{\partial z} (y^2 \cos x + z^3) \right] + \vec{k} \left[ \frac{\partial}{\partial x} (2y \sin x - 4) - \frac{\partial}{\partial y} (y^2 \cos x + z^3) \right]$$

$$= \vec{i} (0) - \vec{j} (3z^2 - 3z^2) + \vec{k} (2y \cos x - 2y \cos x)$$

$$\nabla \times \vec{F} = 0$$

$\vec{F}$  is irrotational.

Then:

$$\nabla \phi = \vec{i} \frac{\partial \phi}{\partial x} + \vec{j} \frac{\partial \phi}{\partial y} + \vec{k} \frac{\partial \phi}{\partial z}$$

$$\vec{F} = (y^2 \cos x + z^3) \vec{i} + (2y \sin x - 4) \vec{j} + 3xz^2 \vec{k}$$

Equating the both coefficient  $\vec{i}, \vec{j}, \vec{k}$

$$\frac{\partial \phi}{\partial x} = y^2 \cos x + z^3 \quad \text{--- (1)}$$

$$\frac{\partial \phi}{\partial y} = 2y \sin x - 4 \quad \text{--- (2)}$$

$$\frac{\partial \phi}{\partial z} = 3xz^2 \quad \text{--- (3)}$$

Integrating w.r to  $x$  in (1)

$$\int d\phi = \int (y^2 \cos x + z^3) dx$$

$$\phi = y^2 \sin x + xz^3 + C \quad \text{--- (4)}$$

Integrating w.r to  $y$  in (2)

$$\int d\phi = \int (2y \sin x - 4) dy$$

$$\phi = \frac{2y^2 \sin x}{2} - 4y$$

$$\phi = y^2 \sin x + 4y + C \quad \text{--- (5)}$$

Integrating w.r to  $z$  in (3)

$$\int d\phi = \int (3xz^2) dz$$

$$\phi = \frac{3xz^3}{3}$$

$$\phi = xz^3 + C \quad \text{--- (6)}$$

Let: From (4), (5), (6)

$$\phi = y^2 \sin x + xz^3 - 4y + C$$

Hence showed

5. Show that  $r^n \vec{r}$  is an irrotational vector for any value of  $n$  but it is solenoidal only if  $n=3$

Let:

$$\vec{r} = x\vec{i} + y\vec{j} + z\vec{k}$$

$$|\vec{r}| = \sqrt{x^2 + y^2 + z^2} \Rightarrow r^2 = x^2 + y^2 + z^2$$

$$r^n = (x^2 + y^2 + z^2)^{n/2}$$

$$r^n \vec{r} = r^n (x\vec{i} + y\vec{j} + z\vec{k})$$

$$\nabla \times (r^n \vec{r}) = \begin{vmatrix} \vec{i} & \vec{j} & \vec{k} \\ \frac{\partial}{\partial x} & \frac{\partial}{\partial y} & \frac{\partial}{\partial z} \\ r^n x & r^n y & r^n z \end{vmatrix}$$

Let:  $r^2 = x^2 + y^2 + z^2$

$$r \frac{\partial r}{\partial x} = x \quad \left| \quad r \frac{\partial r}{\partial y} = y \quad \right| \quad r \frac{\partial r}{\partial z} = z$$

$$\frac{\partial r}{\partial x} = \frac{x}{r} \quad \left| \quad \frac{\partial r}{\partial y} = \frac{y}{r} \quad \right| \quad \frac{\partial r}{\partial z} = \frac{z}{r}$$

$$= \vec{i} \left[ \frac{\partial}{\partial y} (r^n z) - \frac{\partial}{\partial z} (r^n y) \right] - \vec{j} \left[ \frac{\partial}{\partial x} (r^n z) - \frac{\partial}{\partial z} (r^n x) \right]$$

$$+ \vec{k} \left[ \frac{\partial}{\partial x} (r^n y) - \frac{\partial}{\partial y} (r^n x) \right]$$

$$= \vec{i} \left[ z n r^{n-1} \frac{\partial r}{\partial y} - y n r^{n-1} \frac{\partial r}{\partial z} \right] - \vec{j} \left[ z n r^{n-1} \frac{\partial r}{\partial x} - x n r^{n-1} \frac{\partial r}{\partial z} \right]$$

$$- \vec{k} \left[ y n r^{n-1} \frac{\partial r}{\partial x} - x n r^{n-1} \frac{\partial r}{\partial y} \right]$$

$$= \vec{i} \left[ z n r^{n-1} \left( \frac{y}{r} \right) - y n r^{n-1} \left( \frac{z}{r} \right) \right] - \vec{j} \left[ z n r^{n-1} \left( \frac{x}{r} \right) - x n r^{n-1} \left( \frac{z}{r} \right) \right]$$

$$+ \vec{k} \left[ y n r^{n-1} \left( \frac{x}{r} \right) - x n r^{n-1} \left( \frac{y}{r} \right) \right]$$

$$= 0$$

$r^n \vec{r}$  is irrotational for all values of  $n$

$$\nabla \cdot (r^n \vec{r}) = \left( \vec{i} \frac{\partial}{\partial x} + \vec{j} \frac{\partial}{\partial y} + \vec{k} \frac{\partial}{\partial z} \right) \cdot (r^n (x\vec{i} + y\vec{j} + z\vec{k}))$$

$$= \frac{\partial}{\partial x} r^n x + \frac{\partial}{\partial y} r^n y + \frac{\partial}{\partial z} r^n z$$

$$= x^n + xnx^{n-1} \frac{\partial x}{\partial x} + x^n + ynx^{n-1} \frac{\partial x}{\partial y} + x^n + znx^{n-1} \frac{\partial x}{\partial z}$$

$$= 3x^n + xnx^{n-1} \frac{x}{x} + ynx^{n-1} \frac{y}{y} + znx^{n-1} \frac{z}{z}$$

$$= 3x^n + nx^{n-1} x^{-1} x^2 + nx^{n-1} x^{-1} y^2 + nx^{n-1} x^{-1} z^2$$

$$= 3x^n + nx^{n-2} x^2 + nx^{n-2} y^2 + nx^{n-2} z^2$$

$$= 3x^n + nx^{n-2} [x^2 + y^2 + z^2]$$

$$= 3x^n + nx^{n-2} (x^2)$$

$$= 3x^n + nx^n$$

$$\nabla \cdot (x^n \vec{r}) = (3+n)x^n$$

$\nabla \cdot x^n \vec{r} = 0$  it is solenoidal

$$(3+n)x^n = 0$$

$$3+n=0$$

$$\boxed{n=-3}$$

Hence showed